Lots more work on shuffling stutter/mumble closed languages

Models/Stutter_Language.thy
@@ -46,10 +46,48 @@ proof (auto simp add: FIN_def Stutter_def)
 qed
 
 lemma stutter_trans: "xs \<in> stutter ys \<Longrightarrow> ys \<in> stutter zs \<Longrightarrow> xs \<in> stutter zs"
-  sorry
+proof (induct xs rule: stutter.induct)
+  case (self \<sigma>)
+  thus ?case
+    by (metis lappend_code(1) stutter.stutter)
+next
+  case (stutter ws vs \<sigma>)
+  from stutter(2)[OF stutter(3)]
+  show ?case
+    by (rule stutter.stutter)
+next
+  case (mumble ws \<sigma> \<sigma>' \<sigma>'' vs)
+  from mumble(2)[OF mumble(3)]
+  show ?case
+    by (rule stutter.mumble)
+qed
 
 lemma stutter_lappend: "xs \<in> stutter xs' \<Longrightarrow> ys \<in> stutter ys' \<Longrightarrow> (xs \<frown> ys) \<in> stutter (xs' \<frown> ys')"
-  sorry
+proof (induct xs rule: stutter.induct)
+  case (self \<sigma>)
+  thus ?case
+  proof (induct ys rule: stutter.induct)
+    case (self \<sigma>')
+    show ?case
+      by (metis lappend_code(2) stutter.self stutter.stutter)
+  next
+    case (stutter ws vs \<sigma>')
+    thus ?case
+      by (metis lappend_assoc stutter.stutter)
+  next
+    case (mumble ws \<sigma>' \<sigma>'' \<sigma>''' vs)
+    thus ?case
+      by (metis lappend_assoc stutter.mumble)
+  qed
+next
+  case (stutter ws vs \<sigma>')
+  thus ?case
+    by (metis lappend_assoc lappend_code(2) stutter.stutter)
+next
+  case (mumble ws \<sigma> \<sigma>' \<sigma>'' vs)
+  thus ?case
+    by (metis lappend_assoc lappend_code(2) stutter.mumble)
+qed
 
 lemma Stutter_iso: "X \<subseteq> Y \<Longrightarrow> X\<^sup>\<dagger> \<subseteq> Y\<^sup>\<dagger>"
   by (auto simp add: Stutter_def)
@@ -107,8 +145,13 @@ lemma stutter_infinite [dest]: "ys \<in> stutter xs \<Longrightarrow> \<not> lfi
 lemma Stutter_l_prod [simp]: "(X \<cdot> Y)\<^sup>\<dagger> = (X\<^sup>\<dagger> \<cdot> Y\<^sup>\<dagger>)\<^sup>\<dagger>"
   sorry
 
-definition ldeleteLeft :: "enat \<Rightarrow> ('a + 'b) llist \<Rightarrow> ('a + 'b) llist" where
-  "ldeleteLeft n xs = ltakeWhile is_right xs \<frown> ltl (ldropWhile is_right xs)"
+primrec ldeleteLeft_nat :: "nat \<Rightarrow> ('a + 'b) llist \<Rightarrow> ('a + 'b) llist" where
+  "ldeleteLeft_nat 0 xs = ltakeWhile is_right xs \<frown> ltl (ldropWhile is_right xs)"
+| "ldeleteLeft_nat (Suc n) xs = ltakeWhile is_right xs \<frown> LCons (lhd (ldropWhile is_right xs)) (ldeleteLeft_nat n (ltl (ldropWhile is_right xs)))"
+
+primrec ldeleteLeft :: "enat \<Rightarrow> ('a + 'b) llist \<Rightarrow> ('a + 'b) llist" where
+  "ldeleteLeft (enat n) xs = ldeleteLeft_nat n xs"
+| "ldeleteLeft \<infinity> xs = xs"
 
 definition linsertLeft :: "enat \<Rightarrow> 'a \<Rightarrow> ('a + 'b) llist \<Rightarrow> ('a + 'b) llist" where
   "linsertLeft n x xs = undefined"
@@ -124,9 +167,300 @@ lemma "stutter xs \<cdot> stutter ys \<subseteq> stutter (xs \<frown> ys)"
   apply (metis lappend_inf stutter.self stutter_lappend)
   by (metis stutter_lappend)
 
+lemma [simp]: "llength xs = \<infinity> \<Longrightarrow> xs \<frown> ys = xs"
+  by (metis lappend_inf llength_eq_infty_conv_lfinite)
+
+lemma [dest!]: "llength xs = \<infinity> \<Longrightarrow> LNil \<in> xs \<sha> ys \<Longrightarrow> False"
+  by (auto simp add: tshuffle_words_def)
+
+notation ltake ("\<up>")
+  and ldrop ("\<down>")
+
+lemma [simp]: "\<up> (llength xs) xs = xs"
+  by (metis ltake_all order_refl)
+
+lemma [simp]: "traj LNil = LNil"
+  by (metis traj_LNil traj_interleave)
+
+lemma [simp]: "traj (LCons (Inl x) xs) = LCons (Inl ()) (traj xs)"
+  by (simp add: traj_def)
+
+lemma [simp]: "traj (LCons (Inr x) xs) = LCons (Inr ()) (traj xs)"
+  by (simp add: traj_def)
+
+lemma LConsl_in_shuffle [dest]: "LCons (Inl x) (xs \<frown> ys) \<in> xs' \<sha> ys' \<Longrightarrow> xs \<frown> ys \<in> ltl xs' \<sha> ys'"
+  by (auto simp add: tshuffle_words_def)
+
+lemma LConsr_in_shuffle [dest]: "LCons (Inr y) (xs \<frown> ys) \<in> xs' \<sha> ys' \<Longrightarrow> xs \<frown> ys \<in> xs' \<sha> ltl ys'"
+  by (auto simp add: tshuffle_words_def)
+
 lemma interleave_append:
-  "xs \<triangleright> t \<frown> t' \<triangleleft> ys = (ltake (llength (\<ll> t)) xs \<triangleright> t \<triangleleft> ltake (llength (\<rr> t)) ys) \<frown> (ldrop (llength (\<ll> t)) xs \<triangleright> t' \<triangleleft> ldrop (llength (\<rr> t)) ys)"
-  sorry
+  assumes "zs \<in> xs \<sha> ys"
+  and "t \<frown> t' = traj zs"
+  shows "xs \<triangleright> t \<frown> t' \<triangleleft> ys = (\<up> (llength (\<ll> t)) xs \<triangleright> t \<triangleleft> \<up> (llength (\<rr> t)) ys) \<frown> (\<down> (llength (\<ll> t)) xs \<triangleright> t' \<triangleleft> \<down> (llength (\<rr> t)) ys)"
+proof -
+  {
+    assume "\<not> lfinite t"
+    moreover have "\<And>xs ys. \<not> lfinite (xs \<triangleright> t \<triangleleft> ys)"
+      by (metis calculation lfinite_traj)
+    ultimately have ?thesis using assms
+      apply (auto simp add: lappend_inf)
+      apply (subst lappend_inf)
+      apply (simp add: traj_def)
+      apply blast
+      by (metis (lifting, full_types) dual_order.refl ltake_all mem_Collect_eq tshuffle_words_def)
+  }
+  moreover
+  {
+    assume "lfinite t"
+    hence "?thesis" using assms
+    proof (induct t arbitrary: xs ys zs rule: lfinite_induct)
+      case Nil thus ?case by simp
+    next
+      case (Cons w ws)
+      thus ?case
+        apply (cases w)
+        apply (simp add: interleave_left)
+        apply (subgoal_tac "ltl zs \<in> ltl xs \<sha> ys")
+        apply (subgoal_tac "ws \<frown> t' = traj (ltl zs)")
+        apply (metis (hide_lams, no_types) interleave_left ldrop_ltl ltake_ltl)
+        apply (metis interleave_left ltl_simps(2) reinterleave traj_interleave)
+        apply (simp add: tshuffle_words_def)
+        apply (metis interleave_left lefts_LConsl ltl_simps(2) reinterleave rights_LConsl)
+        apply (simp add: interleave_right)
+        apply (subgoal_tac "ltl zs \<in> xs \<sha> ltl ys")
+        apply (subgoal_tac "ws \<frown> t' = traj (ltl zs)")
+        apply (metis (hide_lams, no_types) interleave_right ldrop_ltl ltake_ltl)
+        apply (metis interleave_right ltl_simps(2) reinterleave traj_interleave)
+        apply (simp add: tshuffle_words_def)
+        by (metis interleave_right lefts_LConsr ltl_simps(2) reinterleave rights_LConsr)
+    qed
+  }
+  ultimately show ?thesis by auto
+qed
+
+lemma lefts_ltake_right [simp]: "\<ll> (ltakeWhile is_right xs) = LNil"
+  by (auto dest: lset_ltakeWhileD simp add: lefts_def)
+
+lemma stutter_refl_var: "xs \<noteq> LNil \<Longrightarrow> xs \<in> stutter xs"
+  by (metis neq_LNil_conv stutter_refl)
+
+lemma LCons_lappend_LNil: "LCons y ys = LCons y LNil \<frown> ys"
+  by (metis lappend_code(1) lappend_code(2))
+
+lemma traj_lappend [simp]: "traj (xs \<frown> ys) = traj xs \<frown> traj ys"
+  by (auto simp add: traj_def lmap_lappend_distrib)
+
+lemma [simp]:
+  fixes t :: "(unit + unit) llist"
+  shows "traj t = t"
+  apply (auto simp add: traj_def)
+  apply (subst lmap_ident[symmetric]) back
+  apply (rule lmap2_id)
+proof -
+  fix x :: "(unit + unit)"
+  show "(case x of Inl x \<Rightarrow> Inl x | Inr x \<Rightarrow> Inr x) = x"
+    by (cases x) auto
+qed
+
+lemma intro_traj: "xs \<triangleright> t \<triangleleft> ys = xs \<triangleright> traj t \<triangleleft> ys"
+  by simp
+
+lemma interleave_ldropWhile: "(\<exists>t'\<in>lset t. \<exists>a. t' = Inl a) \<Longrightarrow> ldropWhile is_right (traj t) = LCons (Inl ()) (ltl (ldropWhile is_right (traj t)))"
+  by (metis interleave_ltakeWhile_is_right is_right.simps(2) lappend_LNil2 lappend_ltakeWhile_ldropWhile ldropWhile_rights_not_LNil reinterleave split_llist)
+
+lemma shuffle_lset: "t \<in> xs \<sha> ys \<Longrightarrow> lset t = Inl ` (lset xs) \<union> Inr ` (lset ys)"
+  apply (auto simp add: tshuffle_words_def lefts_def rights_def image_def)
+  apply (metis is_left.simps(2) is_right.simps(2) not_is_left swap.cases unl.simps(1) unr.simps(1))
+  apply (metis is_left.simps(2) obj_sumE unl.simps(1))
+  by (metis is_right.simps(2) obj_sumE unr.simps(1))
+
+lemma lappend_not_LNil_iff [simp]: "xs \<frown> ys \<noteq> LNil \<longleftrightarrow> xs \<noteq> LNil \<or> ys \<noteq> LNil"
+  by (metis LNil_eq_lappend_iff)
+
+lemma [simp]: "lmap f xs \<noteq> LNil \<longleftrightarrow> xs \<noteq> LNil"
+  by (metis LNil_eq_llist_map)
+
+lemma [simp]: "xs \<triangleright> t \<triangleleft> ys \<noteq> LNil \<longleftrightarrow> t \<noteq> LNil"
+  by (metis traj_LNil traj_interleave)
+
+lemma [simp]: "traj t \<noteq> LNil \<longleftrightarrow> t \<noteq> LNil"
+  by (metis reinterleave traj_LNil traj_interleave)
+
+lemma [simp]: "traj (ltakeWhile is_right t) = ltakeWhile is_right (traj t)"
+  by (simp add: traj_def ltakeWhile_lmap)
+
+lemma [simp]: "traj (ltakeWhile is_left t) = ltakeWhile is_left (traj t)"
+  by (simp add: traj_def ltakeWhile_lmap)
+
+lemma [simp]: "traj (ltl t) = ltl (traj t)"
+  by (simp add: traj_def)
+
+lemma [simp]: "traj (ldropWhile is_right t) = ldropWhile is_right (traj t)"
+  by (simp add: traj_def ldropWhile_lmap)
+
+lemma [simp]: "traj (ldropWhile is_left t) = ldropWhile is_left (traj t)"
+  by (simp add: traj_def ldropWhile_lmap)  
+
+lemma [simp]: "lfilter is_left (ltakeWhile is_right t) = LNil"
+  by (metis Not_is_left lfilter_ltakeWhile)
+
+lemma "lfilter is_right (ltakeWhile is_right t) = ltakeWhile is_right t"
+  by (metis Not_is_left lfilter_left_right lfilter_ltakeWhile)
+
+lemma [simp]: "lfilter is_right (ltl (ldropWhile is_right t)) = lfilter is_right (ldropWhile is_right t)"
+  apply (cases "\<exists>t'\<in>lset t. \<exists>a. t' = Inl a")
+  apply (metis is_right.simps(2) lfilter_LCons lhd_ldropWhile llist.collapse ltl_simps(1))
+  apply auto
+  apply (subgoal_tac "ldropWhile is_right t = LNil")
+  apply simp_all
+  apply auto
+  by (metis is_right.simps(1) obj_sumE)
+
+lemma tshuffle_left_LCons: "xs \<in> LCons y ys \<sha> zs \<Longrightarrow> ldeleteLeft_nat 0 xs \<in> ys \<sha> zs"
+  apply (auto simp add: tshuffle_words_def lefts_def rights_def)
+  apply (subst lfilter_lappend_lfinite)
+  apply (metis lappend_inf lappend_ltakeWhile_ldropWhile lefts_def_var lefts_ltake_right llist.distinct(1))
+  apply simp
+  apply (metis Not_is_left ltl_lfilter ltl_lmap ltl_simps(2))
+  apply (subst lfilter_lappend_lfinite)
+  apply (metis lappend_inf lappend_ltakeWhile_ldropWhile lefts_def_var lefts_ltake_right llist.discI)
+  apply simp
+  apply (subst lfilter_lappend_lfinite[symmetric])
+  apply (metis lappend_inf lappend_ltakeWhile_ldropWhile lefts_def_var lefts_ltake_right llist.discI)
+  by (metis lappend_ltakeWhile_ldropWhile)
+
+lemma [simp]: "traj (lmap Inl xs) = lmap (\<lambda>x. Inl ()) xs"
+  by (simp add: traj_def)
+
+lemma [simp]: "ltakeWhile is_right (lmap (\<lambda>x. Inl ()) xs) = LNil"
+  by (metis LNil_preserve is_right.simps(2) llist.exhaust llist.simps(19) ltakeWhile_LCons ltakeWhile_LNil)
+
+lemma [simp]: "ldropWhile is_right (lmap (\<lambda>x. Inl ()) xs) = lmap (\<lambda>x. Inl ()) xs"
+  by (cases xs) simp_all
+
+lemma interleave_only_left_var: "llength t = llength xs \<Longrightarrow> xs \<triangleright> lmap (\<lambda>x. Inl ()) t \<triangleleft> zs = lmap Inl xs"
+  by (metis (full_types) interleave_only_left lmap_const_llength)
+
+lemma stutter_in_left:
+  assumes "t \<in> (xs \<frown> LCons (\<sigma>, \<sigma>) ys) \<sha> zs"
+  shows "lmap \<langle>id,id\<rangle> (xs \<frown> LCons (\<sigma>, \<sigma>) ys \<triangleright> traj t \<triangleleft> zs) \<in> stutter (lmap \<langle>id,id\<rangle> (xs \<frown> ys \<triangleright> ldeleteLeft (llength xs) (traj t) \<triangleleft> zs))"
+proof (cases "llength xs")
+  assume "llength xs = \<infinity>"
+  from this and assms show ?thesis
+    by (auto intro: stutter_refl_var sumlist_cases[of t] simp add: traj_def interleave_left interleave_right)
+next
+  let ?TR = "ltakeWhile is_right"
+  let ?DR = "ldropWhile is_right"
+
+  fix n
+  assume "llength xs = enat n"
+  moreover hence "lmap \<langle>id,id\<rangle> (xs \<frown> LCons (\<sigma>, \<sigma>) ys \<triangleright> traj t \<triangleleft> zs) \<in> stutter (lmap \<langle>id,id\<rangle> (xs \<frown> ys \<triangleright> ldeleteLeft_nat n (traj t) \<triangleleft> zs))" using assms
+  proof (induct n arbitrary: xs t zs)
+    case 0 note zero = this
+    {
+      assume zs_not_LNil: "zs \<noteq> LNil"
+
+      from zero have [simp]: "xs = LNil"
+        by (metis llength_eq_0 zero_enat_def)
+      hence t_shuffle: "t \<in> LCons (\<sigma>, \<sigma>) ys \<sha> zs"
+        by (metis zero(2) lappend_code(1))
+      hence t'_shuffle: "ldeleteLeft_nat 0 t \<in> ys \<sha> zs"
+        by (metis tshuffle_left_LCons)
+      from t_shuffle have t_not_LNil: "t \<noteq> LNil"
+        by (auto simp add: tshuffle_words_def)
+      from t_shuffle and zs_not_LNil have ltl_t_not_LNil: "ltl t \<noteq> LNil"
+        apply (auto simp add: tshuffle_words_def rights_def lefts_def)
+        by (metis (lifting) LNil_preserve lefts_def_var lefts_ltake_right lfilter_LCons lfilter_LNil llist.collapse llist.distinct(1) ltakeWhile_LCons ltakeWhile_eq_LNil_iff t_not_LNil)
+
+      have "lmap \<langle>id,id\<rangle> (LCons (\<sigma>, \<sigma>) ys \<triangleright> traj t \<triangleleft> zs) = lmap \<langle>id,id\<rangle> (LCons (\<sigma>,\<sigma>) ys \<triangleright> ?TR (traj t) \<frown> ?DR (traj t) \<triangleleft> zs)"
+        by (metis lappend_ltakeWhile_ldropWhile)
+      also have "... = lmap \<langle>id,id\<rangle> ((LNil \<triangleright> ?TR (traj t) \<triangleleft> \<up> (llength (\<rr> (?TR (traj t)))) zs) \<frown>
+                                    (LCons (\<sigma>,\<sigma>) ys \<triangleright> ?DR (traj t) \<triangleleft> \<down> (llength (\<rr> (?TR (traj t)))) zs))"
+        apply (subst intro_traj)
+        apply (subst traj_lappend)
+        apply (subst interleave_append[OF t_shuffle])
+        apply (metis intro_traj lappend_ltakeWhile_ldropWhile traj_interleave)
+        by simp
+      also have "... = lmap \<langle>id,id\<rangle> ((LNil \<triangleright> ?TR (traj t) \<triangleleft> \<up> (llength (\<rr> (?TR (traj t)))) zs) \<frown>
+                                     LCons (Inl (\<sigma>,\<sigma>)) (ys \<triangleright> ltl (?DR (traj t)) \<triangleleft> \<down> (llength (\<rr> (?TR (traj t)))) zs))"
+        apply (subst interleave_ldropWhile)
+        apply (subst shuffle_lset[OF t_shuffle])
+        by (simp_all add: interleave_left)
+      also have "... = lmap \<langle>id,id\<rangle> (LNil \<triangleright> ?TR (traj t) \<triangleleft> \<up> (llength (\<rr> (?TR (traj t)))) zs) \<frown>
+                       LCons (\<sigma>,\<sigma>) (lmap \<langle>id,id\<rangle> (ys \<triangleright> ltl (?DR (traj t)) \<triangleleft> \<down> (llength (\<rr> (?TR (traj t)))) zs))"
+        by (simp add: lmap_lappend_distrib)
+      also have "... \<in> stutter (lmap \<langle>id,id\<rangle> (ys \<triangleright> ldeleteLeft_nat 0 (traj t) \<triangleleft> zs))"
+        apply (rule stutter)
+        apply (simp only: ldeleteLeft_nat.simps)
+        apply (subst interleave_append[OF t'_shuffle])
+        apply simp
+        apply (simp only: lefts_ltake_right llength_LNil ltake_0 ldrop_0 lmap_lappend_distrib)
+        apply (rule stutter_refl_var)
+        apply simp
+        apply (rule sumlist_cases[of t])
+        apply simp
+        apply (metis ltl_simps(2) ltl_t_not_LNil)
+        apply simp
+        by (metis t_not_LNil)
+      finally have ?case
+          by auto
+    }
+    moreover
+    {
+      assume zs_LNil: "zs = LNil"
+      from zero have [simp]: "xs = LNil"
+        by (metis llength_eq_0 zero_enat_def)
+      from zs_LNil and zero have ?case
+        by (simp add: interleave_only_left interleave_left)
+    }
+    ultimately show ?case
+      by (cases zs) simp_all
+  next
+    case (Suc n)
+
+    from Suc(2) have xs_lfinite: "lfinite xs"
+      by (metis lfinite_conv_llength_enat)
+
+    from Suc obtain x' and xs' where xs_def: "xs = LCons x' xs'"
+      by (cases xs) (auto simp add: eSuc_enat[symmetric])
+    hence xs'_len: "llength xs' = enat n"
+      by (metis Suc.prems(1) co.enat.inject eSuc_enat llength_LCons)
+
+    have "lmap \<langle>id,id\<rangle> (xs \<frown> LCons (\<sigma>,\<sigma>) ys \<triangleright> traj t \<triangleleft> zs) = lmap \<langle>id,id\<rangle> (xs \<frown> LCons (\<sigma>,\<sigma>) ys \<triangleright> ?TR (traj t) \<frown> ?DR (traj t) \<triangleleft> zs)"
+      by (metis lappend_ltakeWhile_ldropWhile)
+    also have "... = lmap \<langle>id,id\<rangle> ((LNil \<triangleright> ?TR (traj t) \<triangleleft> \<up> (llength (\<rr> (?TR (traj t)))) zs) \<frown>
+                                  (xs \<frown> LCons (\<sigma>, \<sigma>) ys \<triangleright> ?DR (traj t) \<triangleleft> \<down> (llength (\<rr> (?TR (traj t)))) zs))"
+      sorry
+    also have "... = lmap \<langle>id,id\<rangle> ((LNil \<triangleright> ?TR (traj t) \<triangleleft> \<up> (llength (\<rr> (?TR (traj t)))) zs) \<frown>
+                                  (xs \<frown> LCons (\<sigma>, \<sigma>) ys \<triangleright> LCons (Inl ()) (ltl (?DR (traj t))) \<triangleleft> \<down> (llength (\<rr> (?TR (traj t)))) zs))"
+        apply (subst interleave_ldropWhile)
+        apply (subst shuffle_lset[OF Suc(3)])
+        apply auto
+        apply (rule_tac x = "Inl (\<sigma>,\<sigma>)" in bexI)
+        apply auto
+        apply (subgoal_tac "lfinite xs")
+        apply (metis imageI in_lset_lappend_iff lset_intros(1))
+        by (metis xs_lfinite)
+    also have "... = lmap \<langle>id,id\<rangle> ((LNil \<triangleright> ?TR (traj t) \<triangleleft> \<up> (llength (\<rr> (?TR (traj t)))) zs) \<frown>
+                                  LCons (Inl x') (xs' \<frown> LCons (\<sigma>, \<sigma>) ys \<triangleright> ltl (?DR (traj t)) \<triangleleft> \<down> (llength (\<rr> (?TR (traj t)))) zs))"
+      by (metis (hide_lams, no_types) calculation interleave_left lappend_code(2) lhd_LCons ltl_simps(2) xs_def)
+    also have "... = lmap \<langle>id,id\<rangle> (LNil \<triangleright> ?TR (traj t) \<triangleleft> \<up> (llength (\<rr> (?TR (traj t)))) zs) \<frown>
+                     LCons x' (lmap \<langle>id,id\<rangle> (xs' \<frown> LCons (\<sigma>, \<sigma>) ys \<triangleright> ltl (?DR (traj t)) \<triangleleft> \<down> (llength (\<rr> (?TR (traj t)))) zs))"
+      by (simp add: lmap_lappend_distrib)
+    also have "... \<in> stutter (lmap \<langle>id,id\<rangle> (xs \<frown> ys \<triangleright> ldeleteLeft_nat (Suc n) (traj t) \<triangleleft> zs))"
+      apply (simp only: ldeleteLeft_nat.simps)
+      apply (subst interleave_append)
+      prefer 3
+      apply (simp only: lmap_lappend_distrib)
+      apply (rule stutter_lappend)
+      sorry
+    finally show ?case
+      by auto
+  qed
+  ultimately show ?thesis
+    by simp
+qed
 
 lemma tshuffle_stutter: "\<Union>{lmap \<langle>id,id\<rangle> ` (xs' \<sha> ys)|xs'. xs' \<in> stutter xs} \<subseteq> (lmap \<langle>id,id\<rangle> ` (xs \<sha> ys))\<^sup>\<dagger>"
 proof -
